Use \tau

src/statics.lean
@@ -5,8 +5,8 @@ inductive has_typ: exp -> typ -> Prop
 | true: has_typ exp.true typ.bool
 | false: has_typ exp.false typ.bool
 | if_
-    (e1: exp) (e2: exp) (e3: exp) (t: typ):
+    (e1: exp) (e2: exp) (e3: exp) (τ: typ):
     has_typ e1 typ.bool ->
-    has_typ e2 t ->
-    has_typ e3 t ->
-    has_typ (exp.if_ e1 e2 e3) t
+    has_typ e2 τ ->
+    has_typ e3 τ ->
+    has_typ (exp.if_ e1 e2 e3) τ
