src/helpers.lean
@@ -2,8 +2,8 @@ import statics
 import dynamics
 
 theorem inversion_if_e1
-  (e1: exp) (e2: exp) (e3: exp) (t: typ)
-  (typing: has_typ (exp.if_ e1 e2 e3) t)
+  (e1: exp) (e2: exp) (e3: exp) (τ: typ)
+  (typing: has_typ (exp.if_ e1 e2 e3) τ)
   : has_typ e1 typ.bool :=
 begin
   cases typing,
@@ -11,18 +11,18 @@ begin
 end
 
 theorem inversion_if_e2
-  (e1: exp) (e2: exp) (e3: exp) (t: typ)
-  (typing: has_typ (exp.if_ e1 e2 e3) t)
-  : has_typ e2 t :=
+  (e1: exp) (e2: exp) (e3: exp) (τ: typ)
+  (typing: has_typ (exp.if_ e1 e2 e3) τ)
+  : has_typ e2 τ :=
 begin
   cases typing,
   exact typing_a_1,
 end
 
 theorem inversion_if_e3
-  (e1: exp) (e2: exp) (e3: exp) (t: typ)
-  (typing: has_typ (exp.if_ e1 e2 e3) t)
-  : has_typ e3 t :=
+  (e1: exp) (e2: exp) (e3: exp) (τ: typ)
+  (typing: has_typ (exp.if_ e1 e2 e3) τ)
+  : has_typ e3 τ :=
 begin
   cases typing,
   exact typing_a_2,
